theories/Unification.v
@@ -29,7 +29,12 @@
 From Coq Require Import
      Arith.PeanoNat
      Classes.CRelationClasses
-     Program.Tactics.
+     Classes.Equivalence
+     Classes.Morphisms
+     Program.Equality
+     Program.Tactics
+     Setoid
+     Recdef.
 From Equations Require Import
      Equations.
 From Equations.Type Require
@@ -38,82 +43,256 @@ From Equations.Type Require
 From Equations.Prop Require
      Classes.
 From MasterThesis Require Import
-     Context Environment Prelude.
+     Context Environment Prelude STLC.
 Import ctx.
 Import ctx.notations.
 Import SigTNotations.
 
 Set Implicit Arguments.
 
-Definition TYPE : Type := Ctx nat -> Type.
+Notation World := (Ctx nat).
+Definition TYPE : Type := World -> Type.
 Definition Valid (A : TYPE) : Type :=
-  forall Σ, A Σ.
+  forall w, A w.
 Definition Impl (A B : TYPE) : TYPE :=
-  fun Σ => A Σ -> B Σ.
+  fun w => A w -> B w.
 Definition Forall {I : Type} (A : I -> TYPE) : TYPE :=
   fun w => forall i : I, A i w.
 
+Definition Assignment : TYPE :=
+  env.Env (fun _ => ty).
+Definition Lifted (A : Type) : TYPE :=
+  fun Σ => Assignment Σ -> A.
+
+Notation "⊢ A" := (Valid A) (at level 100).
+Notation "A -> B" := (Impl A B).
+
 Definition Unit : TYPE := fun _ => unit.
-Definition Option (A : TYPE) : TYPE := fun Σ => option (A Σ).
-Definition Prod (A B : TYPE) : TYPE := fun Σ => prod (A Σ) (B Σ).
-Definition Sum (A B : TYPE) : TYPE := fun Σ => sum (A Σ) (B Σ).
+Definition Option (A : TYPE) : TYPE := fun w => option (A w).
+Definition List (A : TYPE) : TYPE := fun w => list (A w).
+Definition Prod (A B : TYPE) : TYPE := fun w => prod (A w) (B w).
+Definition Sum (A B : TYPE) : TYPE := fun w => sum (A w) (B w).
 
-Inductive Ty (Σ : Ctx nat) : Type :=
-  | t_evar (x : nat) (xIn : x ∈ Σ)
-  | t_bool
-  | t_func (T1 T2 : Ty Σ).
-Arguments t_evar {Σ x} xIn.
-Arguments t_bool {Σ}.
-Arguments t_func {Σ}.
+Local Arguments Ty_hole {Σ i} xIn.
+Local Arguments Ty_bool {Σ}.
+Local Arguments Ty_func {Σ}.
 
-Derive NoConfusion for Ty.
+Derive NoConfusion Subterm for Ty.
+
+Definition Ty_subterm_refl {w} :=
+  Relation_Operators.clos_refl (Ty w) (Ty_subterm (Σ:=w)).
+
+Section DecEquality.
+
+  Local Set Equations With UIP.
+
+  Instance In_eqdec {w} : EqDec (sigT (fun x : nat => In x w)).
+  Proof.
+    intros [x xIn] [y yIn].
+    induction xIn; cbn; destruct (ctx.snocView yIn) as [|y yIn].
+    - left. reflexivity.
+    - right. abstract discriminate.
+    - right. abstract discriminate.
+    - destruct (IHxIn yIn); clear IHxIn; [left|right].
+      + abstract (now dependent elimination e).
+      + abstract (intros e; apply n; clear n;
+                  now dependent elimination e).
+  Defined.
+
+  Instance Ty_eqdec {w} : EqDec (Ty w).
+  Proof.
+    change_no_check (forall x y : Ty w, dec_eq x y).
+    induction x; destruct y; cbn; try (right; abstract discriminate).
+    - left. auto.
+    - apply f_equal2_dec; auto.
+      now intros H%noConfusion_inv.
+    - destruct (eq_dec (i; i0) (i1; i2)).
+      + left. abstract now dependent elimination e.
+      + right. abstract (intros H; apply n; clear n; inversion H; auto).
+  Defined.
+
+End DecEquality.
+#[export] Existing Instance In_eqdec.
+#[export] Existing Instance Ty_eqdec.
+
+Reserved Notation "w1 ⊒ w2" (at level 80).
+Reserved Notation "w1 ⊒⁻ w2" (at level 80).
+Reserved Notation "w1 ⊒ˢ w2" (at level 80).
+
+Definition BoxR (R : Relation.relation World) (A : TYPE) : TYPE :=
+  fun w0 => forall w1, R w0 w1 -> A w1.
+Definition DiamondR (R : Relation.relation World) (A : TYPE) : TYPE :=
+  fun w0 => {w1 & R w0 w1 * A w1}%type.
+Notation "[< R >] A" := (BoxR R A) (at level 9, format "[< R >] A", right associativity).
+
+Definition Later (A : TYPE) : TYPE :=
+  fun w => forall x (xIn : x ∈ w), A (w - x).
+Definition LaterTm (A : TYPE) : TYPE :=
+  fun w => forall x (xIn : x ∈ w), Ty (w - x) -> A (w - x).
+Notation "▻ A" := (Later A) (at level 9, right associativity).
+Notation "► A" := (LaterTm A) (at level 9, right associativity).
+Definition Sooner (A : TYPE) : TYPE :=
+  fun w => sigT (fun x => sigT (fun (xIn : x ∈ w) => A (w - x))).
+Definition SoonerTm (A : TYPE) : TYPE :=
+  fun w => sigT (fun x => sigT (fun (xIn : x ∈ w) => Ty (w - x) * A (w - x)))%type.
+Notation "◅ A" := (Sooner A) (at level 9, right associativity).
+Notation "◄ A" := (SoonerTm A) (at level 9, right associativity).
+
+Section Thick.
+
+  Definition thickIn {w x} (xIn : x ∈ w) (s : Ty (w - x)) :
+    forall y, y ∈ w -> Ty (w - x) :=
+    fun y yIn =>
+      match occurs_check_view xIn yIn with
+      | Same _     => s
+      | Diff _ yIn => Ty_hole yIn
+      end.
+
+  Definition thick : ⊢ Ty -> ►Ty :=
+    fun w =>
+      fix thick (S : Ty w) (x : nat) (xIn : x ∈ w) (T : Ty (w - x)) {struct S} : Ty (w - x) :=
+      match S with
+      | Ty_hole σIn   => thickIn xIn T σIn
+      | Ty_bool       => Ty_bool
+      | Ty_func S1 S2 => Ty_func (thick S1 x xIn T) (thick S2 x xIn T)
+      end.
+
+End Thick.
+
+Section Thin.
+
+  Fixpoint thin {w x} (xIn : x ∈ w) (T : Ty (w - x)) : Ty w :=
+    match T with
+    | Ty_hole yIn => Ty_hole (in_thin xIn yIn)
+    | Ty_bool => Ty_bool
+    | Ty_func T1 T2 => Ty_func (thin xIn T1) (thin xIn T2)
+    end.
+
+  Definition fancy_thin : ⊢ ◅Ty -> Ty :=
+    fun w '(x; (xIn; T)) => thin xIn T.
+
+End Thin.
 
 Module Tri.
 
-  Inductive Tri (Σ : Ctx nat) : Ctx nat -> Set :=
-  | refl      : Tri Σ Σ
-  | cons {Σ' x} (xIn : x ∈ Σ) (t : Ty (Σ - x)%ctx) (ζ : Tri (Σ - x) Σ') : Tri Σ Σ'.
+  Import Coq.Classes.CRelationClasses.
+
+  Inductive Tri (w : World) : World -> Set :=
+  | refl      : w ⊒⁻ w
+  | cons {w' x} (xIn : x ∈ w) (t : Ty (w - x)) (ζ : w - x ⊒⁻ w') : w ⊒⁻ w'
+  where "w1 ⊒⁻ w2" := (Tri w1 w2).
   Global Arguments refl {_}.
   Global Arguments cons {_ _} x {_} t ζ.
 
-  Fixpoint trans [Σ0 Σ1 Σ2] (ζ : Tri Σ0 Σ1) {struct ζ} : Tri Σ1 Σ2 -> Tri Σ0 Σ2 :=
-     match ζ with
-     | refl       => fun ξ => ξ
-     | cons x t ν => fun ξ => cons x t (trans ν ξ)
-     end.
-
-  #[export] Instance preorder_tri : CRelationClasses.PreOrder Tri :=
-    {| PreOrder_Reflexive Σ := refl;
+  Fixpoint trans [w0 w1 w2] (ζ1 : w0 ⊒⁻ w1) {struct ζ1} : w1 ⊒⁻ w2 -> w0 ⊒⁻ w2 :=
+    match ζ1 with
+    | refl        => fun ζ2 => ζ2
+    | cons x t ζ1 => fun ζ2 => cons x t (trans ζ1 ζ2)
+    end.
+  Local Infix "⊙" := trans (at level 60, right associativity).
+  #[export] Instance preorder_tri : PreOrder Tri :=
+    {| PreOrder_Reflexive w := refl;
        PreOrder_Transitive  := trans
     |}.
 
+  Definition single {w} x {xIn : x ∈ w} (t : Ty (w - x)) : w ⊒⁻ w - x :=
+    cons x t refl.
+  Global Arguments single {w} x {xIn} t.
+
+  Lemma trans_refl {w1 w2} (ζ : w1 ⊒⁻ w2) : ζ ⊙ refl = ζ.
+  Proof. induction ζ; cbn; congruence. Qed.
+
+  Lemma trans_assoc {w0 w1 w2 w3} (ζ1 : w0 ⊒⁻ w1) (ζ2 : w1 ⊒⁻ w2) (ζ3 : w2 ⊒⁻ w3) :
+    (ζ1 ⊙ ζ2) ⊙ ζ3 = ζ1 ⊙ (ζ2 ⊙ ζ3).
+  Proof. induction ζ1; cbn; congruence. Qed.
+
+  (* Definition geq {w0 w1} (ζ1 : w0 ⊒⁻ w1) [w2] (ζ2 : w0 ⊒⁻ w2) : Prop := *)
+  (*   exists ζ12 : w1 ⊒⁻ w2, ζ2 = ζ1 ⊙ ζ12. *)
+  (* Notation "ζ1 ≽ ζ2" := (geq ζ1 ζ2) (at level 80). *)
+
+  (* Lemma geq_refl {w1 w2} (ζ : w1 ⊒⁻ w2) : ζ ≽ ζ. *)
+  (* Proof. exists refl. symmetry. apply trans_refl. Qed. *)
+
+  (* Lemma geq_trans {w0 w1 w2 w3} (ζ1 : w0 ⊒⁻ w1) (ζ2 : w0 ⊒⁻ w2) (ζ3 : w0 ⊒⁻ w3) : *)
+  (*   ζ1 ≽ ζ2 -> ζ2 ≽ ζ3 -> ζ1 ≽ ζ3. *)
+  (* Proof. *)
+  (*   intros [ζ12 H12] [ζ23 H23]. exists (ζ12 ⊙ ζ23). *)
+  (*   rewrite H23, H12. apply trans_assoc. *)
+  (* Qed. *)
+
+  (* Lemma geq_precom {w0 w1 w2 w3} (ζ1 : w0 ⊒⁻ w1) (ζ2 : w1 ⊒⁻ w2) (ζ3 : w1 ⊒⁻ w3) : *)
+  (*   ζ2 ≽ ζ3 -> ζ1 ⊙ ζ2 ≽ ζ1 ⊙ ζ3. *)
+  (* Proof. intros [ζ23 ->]. exists ζ23. symmetry. apply trans_assoc. Qed. *)
+
+  (* Lemma geq_max {w1 w2} (ζ : w1 ⊒⁻ w2) : refl ≽ ζ. *)
+  (* Proof. exists ζ. reflexivity. Qed. *)
+
+  (* Lemma geq_extend {w0 w1 w2} (ζ1 : w0 ⊒⁻ w1) (ζ2 : w1 ⊒⁻ w2) : ζ1 ≽ ζ1 ⊙ ζ2. *)
+  (* Proof. now exists ζ2. Qed. *)
+
+  (* Definition geqb1 [w0 z] (zIn : z ∈ w0) (tz : Ty (w0 - z)) [w1] (ζ : w0 ⊒⁻ w1) : *)
+  (*   option (w0 - z ⊒⁻ w1). *)
+  (* Proof. *)
+  (*   rename w1 into wend. *)
+  (*   induction ζ. *)
+  (*   + apply None. *)
+  (*   + rename w' into wend. rename t into tx. *)
+  (*     destruct (occurs_check_view xIn zIn). *)
+  (*     * refine (if Ty_eqdec tx tz then Some ζ else None). *)
+  (*     * rename y into z. rename yIn into zIn. *)
+  (*       specialize (IHζ zIn). *)
+  (*       Check (thick (thin _ tz) _ tx). *)
+  (* Admitted. *)
+
+  (* Fixpoint geqb (w0 w1 : World) (ζ1 : w0 ⊒⁻ w1) {w2} (ζ2 : w0 ⊒⁻ w2) {struct ζ1} : *)
+  (*   option (w1 ⊒⁻ w2) := *)
+  (*   match ζ1 with *)
+  (*   | refl => Some ζ2 *)
+  (*   | cons x t__X ζ1' => *)
+  (*       option.bind (geqb1 _ t__X ζ2) (geqb ζ1') *)
+  (*   end. *)
+
+  (* Lemma geqb_spec {w0 w1} (ζ1 : w0 ⊒⁻ w1) : *)
+  (*   forall [w2] (ζ2 : w0 ⊒ˢ w2), *)
+  (*     Bool.reflect (triangular ζ1 ≽ ζ2) (ζ1 ≽? ζ2). *)
+  (* Proof. *)
+  (*   induction ζ1; cbn [geqb triangular]; intros w2 ζ2. *)
+  (*   - constructor. apply geq_max. *)
+  (*   - destruct Ty_eqdec. *)
+  (*     + destruct (IHζ1 _ (thin xIn ⊙ˢ ζ2)); constructor; clear IHζ1. *)
+  (*       * destruct g as [ζ2']. exists ζ2'. *)
+  (*         rewrite comp_assoc. rewrite <- H. clear - e. *)
+  (*         apply env.lookup_extensional. *)
+  (*         intros y yIn. *)
+  (*         rewrite lookup_comp. *)
+  (*         rewrite lookup_thick. unfold thickIn. *)
+  (*         destruct (occurs_check_view xIn yIn). apply e. *)
+  (*         cbn. rewrite lookup_comp. unfold thin. *)
+  (*         now rewrite env.lookup_tabulate. *)
+  (*       * intros [ζ2' ->]. apply n. clear n. exists ζ2'. *)
+  (*         rewrite <- ?comp_assoc. *)
+  (*         rewrite comp_thin_thick. *)
+  (*         rewrite comp_id_left. *)
+  (*         reflexivity. *)
+  (*     + constructor. intros [ζ2' ->]. apply n. clear n. *)
+  (*       rewrite <- ?comp_assoc. *)
+  (*       rewrite comp_thin_thick. *)
+  (*       rewrite comp_id_left. *)
+  (*       cbn. rewrite ?lookup_comp, lookup_thick. *)
+  (*       unfold thickIn. rewrite occurs_check_view_refl. *)
+  (*       now rewrite subst_comp. *)
+  (* Qed. *)
+
 End Tri.
-Notation "Σ1 ⊒ Σ2" := (Tri.Tri Σ1 Σ2) (at level 80).
+Notation "w1 ⊒⁻ w2" := (Tri.Tri w1 w2) (at level 80).
+Infix "⊙" := Tri.trans (at level 60, right associativity).
 
 Definition Box (A : TYPE) : TYPE :=
-  fun w0 => forall w1, w0 ⊒ w1 -> A w1.
-
-Unset Printing Notations.
+  fun w0 => forall w1, w0 ⊒⁻ w1 -> A w1.
 Definition Diamond (A : TYPE) : TYPE :=
-  fun w0 => {w1 : Ctx nat & ((w0 ⊒ w1) * A w1)}%type.
-
-Print Diamond.
-
+  fun w0 => {w1 : World & ((w0 ⊒⁻ w1) * A w1)}%type.
 Definition DiamondT (M : TYPE -> TYPE) : TYPE -> TYPE :=
-  fun A => M (fun w0 => {w1 : Ctx nat & ((w0 ⊒ w1) * A w1)}%type).
-
-Definition Later (A : TYPE) : TYPE :=
-  fun Γ => forall x (xIn : x ∈ Γ), A (Γ - x).
-Definition LaterTm (A : TYPE) : TYPE :=
-  fun Γ => forall x (xIn : x ∈ Γ), Ty (Γ - x) -> A (Γ - x).
-Definition Sooner (A : TYPE) : TYPE :=
-  fun Γ => sigT (fun x => sigT (fun (xIn : x ∈ Γ) => A (Γ - x))).
-Definition SoonerTm (A : TYPE) : TYPE :=
-  fun Γ => sigT (fun x => sigT (fun (xIn : x ∈ Γ) => Ty (Γ - x) * A (Γ - x)))%type.
-
-
-Notation "◅ A" := (Sooner A) (at level 9, right associativity).
-Notation "◄ A" := (SoonerTm A) (at level 9, right associativity).
+  fun A => M (fun w0 => {w1 : World & ((w0 ⊒⁻ w1) * A w1)}%type).
 
 Notation "□ A" := (Box A) (at level 9, format "□ A", right associativity).
 Notation "◇ A" := (DiamondT id A) (at level 9, format "◇ A", right associativity).
@@ -121,24 +300,31 @@ Notation "? A" := (Option A) (at level 9, format "? A", right associativity).
 Notation "◆ A" := (DiamondT Option A) (at level 9, format "◆ A", right associativity).
 Notation "A * B" := (Prod A B).
 
-Notation "⊢ A" := (Valid A) (at level 100).
-Notation "A -> B" := (Impl A B).
 Notation "'∀' x .. y , P " :=
   (Forall (fun x => .. (Forall (fun y => P)) ..))
     (at level 99, x binder, y binder, right associativity).
-Notation "▻ A" := (Later A) (at level 9, right associativity).
-Notation "► A" := (LaterTm A) (at level 9, right associativity).
 
 Section Löb.
 
-  Context (P : TYPE) (step : ⊢ ▻P -> P).
+  Context (A : TYPE) (step : ⊢ ▻A -> A).
 
   Obligation Tactic := auto using Nat.eq_le_incl, length_remove.
-  Equations(noeqns) Löb {Σ : Ctx nat} : P Σ by wf (length Σ) :=
-  Löb := step (fun _ _ => Löb).
+  Equations Löbaux {w : World} : A w by wf (length w) :=
+  Löbaux := step (fun _ _ => Löbaux).
+  Local Arguments Löbaux : clear implicits.
+
+  Transparent Löbaux.
+  Definition Löb : ⊢ A := Löbaux.
+
+  Context (P : forall w : World, A w -> Type).
+  Context (pstep : forall w,
+        (forall x (xIn : x ∈ w), P (Löb (w - x))) ->
+        P (step (fun x xIn => Löb (w - x)))).
+
+  Definition Löb_elim : forall w, P (Löb w) :=
+    Löbaux_elim P pstep.
 
 End Löb.
-Arguments Löb P step Σ : clear implicits.
 
 Definition K {A B} :
   ⊢ □(A -> B) -> (□A -> □B) :=
@@ -153,74 +339,223 @@ Definition four {A} :
     a w2 (Tri.trans ω01 ω12).
 Global Arguments four : simpl never.
 Definition D {A} : ⊢ □A -> ◇A :=
-  fun Σ a => existT _ Σ (Tri.refl, T a).
+  fun w a => existT _ w (Tri.refl, T a).
 
 Definition box2later {A} : ⊢ □A -> ►A.
-  intros Σ a x xIn t. apply a. econstructor.
+  intros w a x xIn t. apply a. econstructor.
   apply t. constructor.
 Defined.
 
-Definition sooner2diamond {A} : ⊢ ◄A -> ◇A.
-  intros Σ a. destruct a as [σ [σIn [t a]]].
-  econstructor. split; try eassumption.
-  econstructor 2. auto. constructor 1.
-Defined.
+Definition sooner2diamond {A} : ⊢ ◄A -> ◇A :=
+  fun w a =>
+    match a with
+      existT _ x (existT _ xIn (t , a)) =>
+      existT _ (w - x) (pair (Tri.single x t) a)
+    end.
 
 Definition sooner2diamondtm {A} : ⊢ ◄A -> ◆A.
-  intros Σ a. destruct a as [σ [σIn [t a]]].
+  intros w a. destruct a as [σ [σIn [t a]]].
   constructor.
   econstructor. split; try eassumption.
   econstructor 2. auto. constructor 1.
 Defined.
 
 Definition η {A} : ⊢ A -> ◆A :=
-  fun Σ a => Some (existT _ Σ (Tri.refl, a)).
-Arguments η {A Σ} a.
+  fun w a => Some (existT _ w (Tri.refl, a)).
+Arguments η {A w} a.
 
-Definition η1 {A} {Σ x} {xIn : x ∈ Σ} (t : Ty (Σ - x)) (a : A (Σ - x)) : ◆A Σ :=
+Definition η1 {A} {w x} {xIn : x ∈ w} (t : Ty (w - x)) (a : A (w - x)) : ◆A w :=
   sooner2diamondtm (existT _ x (existT _ xIn (t, a))).
 
-Section Thick.
 
-  Definition thick : ⊢ Ty -> ►Ty :=
-    fun Σ =>
-      fix thick (S : Ty Σ) (x : nat) (xIn : x ∈ Σ) (T : Ty (Σ - x)) {struct S} : Ty (Σ - x) :=
+(* Arguments thick {_} s x {_} u. *)
+(* Notation "s [ x ↦ u ]" := (thick s x u) *)
+(*   (at level 8, left associativity, *)
+(*    format "s [ x ↦ u ]"). *)
+
+
+(* Lemma thin_thick {w y} (yIn : y ∈ w) (s t : Ty (w - y)) : *)
+(*   (thin yIn t)[y↦s] = t. *)
+(* Proof. *)
+(*   induction t; cbn; f_equal; auto. unfold thickIn. *)
+(*   now rewrite occurs_check_view_thin. *)
+(* Qed. *)
+
+Module Sub.
+
+  Definition Sub (w1 w2 : World) : Type :=
+    @env.Env nat (fun _ => Ty w2) w1.
+  Local Notation "w1 ⊒ˢ w2" := (Sub w1 w2).
+
+  Definition Box (A : TYPE) : TYPE :=
+    fun w0 => forall w1, w0 ⊒ˢ w1 -> A w1.
+  Local Notation "□ A" := (Box A) (at level 9, format "□ A", right associativity).
+
+  Definition subst : ⊢ Ty -> □Ty :=
+    fun w1 =>
+      fix subst (S : Ty w1) {w2} (ζ : w1 ⊒ˢ w2) {struct S} : Ty w2 :=
       match S with
-      | t_evar σIn   => match occurs_check_view xIn σIn with
-                        | Same _     => T
-                        | Diff _ yIn => t_evar yIn
-                        end
-      | t_bool       => t_bool
-      | t_func S1 S2 => t_func (thick S1 x xIn T) (thick S2 x xIn T)
+      | Ty_hole σIn   => env.lookup ζ σIn
+      | Ty_bool       => Ty_bool
+      | Ty_func S1 S2 => Ty_func (subst S1 ζ) (subst S2 ζ)
       end.
 
-End Thick.
+  Definition id {w} : w ⊒ˢ w :=
+    env.tabulate (fun _ => Ty_hole).
+  Definition thick {w x} (xIn : x ∈ w) (s : Ty (w - x)) : w ⊒ˢ w - x :=
+    env.tabulate (thickIn xIn s).
+  Definition thin {w x} (xIn : x ∈ w) : w - x ⊒ˢ w :=
+    env.tabulate (fun y yIn => Ty_hole (in_thin xIn yIn)).
+  Definition comp {w0 w1 w2} (ζ1 : w0 ⊒ˢ w1) (ζ2 : w1 ⊒ˢ w2) : w0 ⊒ˢ w2 :=
+    env.map (fun _ t => subst t ζ2) ζ1.
+  Local Infix "⊙ˢ" := comp (at level 60, right associativity).
 
-Arguments thick {_} s x {_} u.
-Notation "s [ x ↦ u ]" := (thick s x u)
-  (at level 8, left associativity,
-   format "s [ x ↦ u ]").
-
-Section Thin.
-
-  Fixpoint thin {Σ x} (xIn : x ∈ Σ) (T : Ty (Σ - x)) : Ty Σ :=
-    match T with
-    | t_evar yIn => t_evar (in_thin xIn yIn)
-    | t_bool => t_bool
-    | t_func T1 T2 => t_func (thin xIn T1) (thin xIn T2)
+  Fixpoint triangular {w1 w2} (ζ : w1 ⊒⁻ w2) : w1 ⊒ˢ w2 :=
+    match ζ with
+    | Tri.refl       => id
+    | Tri.cons x t ζ => comp (thick _ t) (triangular ζ)
     end.
 
-  Definition fancy_thin : ⊢ ◅Ty -> Ty :=
-    fun Σ '(x; (xIn; T)) => thin xIn T.
+  Lemma lookup_id {w x} (xIn : x ∈ w)  :
+    env.lookup id xIn = Ty_hole xIn.
+  Proof. unfold id. now rewrite env.lookup_tabulate. Qed.
 
-End Thin.
+  Lemma lookup_comp {w1 w2 w3 x} (xIn : x ∈ w1) (ζ1 : w1 ⊒ˢ w2) (ζ2 : w2 ⊒ˢ w3) :
+    env.lookup (comp ζ1 ζ2) xIn = subst (env.lookup ζ1 xIn) ζ2.
+  Proof. unfold comp. now rewrite env.lookup_map. Qed.
 
-Lemma thin_thick {Σ y} (yIn : y ∈ Σ) (s t : Ty (Σ - y)) :
-  (thin yIn t)[y↦s] = t.
-Proof.
-  induction t; cbn; f_equal; auto.
-  now rewrite occurs_check_view_thin.
-Qed.
+  Lemma lookup_thin {w x y} (xIn : x ∈ w) (yIn : y ∈ w - x) :
+    env.lookup (thin xIn) yIn = Ty_hole (in_thin xIn yIn).
+  Proof. unfold thin. now rewrite env.lookup_tabulate. Qed.
+
+  Lemma lookup_thick {w x y} (xIn : x ∈ w) (t : Ty _) (yIn : y ∈ w) :
+    env.lookup (thick xIn t) yIn = thickIn xIn t yIn.
+  Proof. unfold thick. now rewrite env.lookup_tabulate. Qed.
+
+  Lemma subst_id {w} (t : Ty w) :
+    subst t id = t.
+  Proof. induction t; cbn; f_equal; now rewrite ?lookup_id. Qed.
+
+  Lemma subst_comp {w1} (t : Ty w1) {w2 w3} (ζ2 : w2 ⊒ˢ w3) (ζ1 : w1 ⊒ˢ w2) :
+    subst t (comp ζ1 ζ2) = subst (subst t ζ1) ζ2.
+  Proof. induction t; cbn; f_equal; now rewrite ?lookup_comp. Qed.
+
+  Lemma comp_assoc {w1 w2 w3 w4} (ζ1 : w1 ⊒ˢ w2) (ζ2 : w2 ⊒ˢ w3) (ζ3 : w3 ⊒ˢ w4) :
+    comp (comp ζ1 ζ2) ζ3 = comp ζ1 (comp ζ2 ζ3).
+  Proof.
+    apply env.lookup_extensional. intros x xIn.
+    now rewrite ?lookup_comp, subst_comp.
+  Qed.
+
+  Lemma comp_id_left {w1 w2} (ζ : w1 ⊒ˢ w2) : comp id ζ = ζ.
+  Proof.
+    apply env.lookup_extensional. intros x xIn.
+    now rewrite lookup_comp, lookup_id.
+  Qed.
+
+  Lemma comp_id_right {w1 w2} (ζ : w1 ⊒ˢ w2) :
+    comp ζ id = ζ.
+  Proof.
+    apply env.lookup_extensional. intros x xIn.
+    now rewrite lookup_comp, subst_id.
+  Qed.
+
+  Lemma triangular_trans {w0 w1 w2} (ζ01 : w0 ⊒⁻ w1) (ζ12 : w1 ⊒⁻ w2) :
+    triangular (Tri.trans ζ01 ζ12) =
+      comp (triangular ζ01) (triangular ζ12).
+  Proof.
+    induction ζ01; cbn [triangular Tri.trans].
+    - now rewrite comp_id_left.
+    - now rewrite comp_assoc, IHζ01.
+  Qed.
+
+  Lemma comp_thin_thick {w x} (xIn : x ∈ w) (t : Ty (w - x)) :
+    comp (thin xIn) (thick xIn t) = id.
+  Proof.
+    apply env.lookup_extensional. intros y yIn.
+    rewrite lookup_comp, lookup_id, lookup_thin. cbn.
+    rewrite lookup_thick. unfold thickIn.
+    now rewrite occurs_check_view_thin.
+  Qed.
+
+  Lemma subst_thin {w x} (xIn : x ∈ w) (T : Ty (w - x)) :
+    Unification.thin xIn T = subst T (thin xIn).
+  Proof. induction T; cbn; f_equal; now rewrite ?lookup_thin. Qed.
+
+  Definition geq {w0 w1} (ζ1 : w0 ⊒ˢ w1) [w2] (ζ2 : w0 ⊒ˢ w2) : Prop :=
+    exists ζ12 : w1 ⊒ˢ w2, ζ2 = ζ1 ⊙ˢ ζ12.
+  Notation "ζ1 ≽ ζ2" := (geq ζ1 ζ2) (at level 80).
+
+  Lemma geq_refl {w1 w2} (ζ : w1 ⊒ˢ w2) : ζ ≽ ζ.
+  Proof. exists Sub.id. symmetry. apply Sub.comp_id_right. Qed.
+
+  Lemma geq_trans {w0 w1 w2 w3} (ζ1 : w0 ⊒ˢ w1) (ζ2 : w0 ⊒ˢ w2) (ζ3 : w0 ⊒ˢ w3) :
+    ζ1 ≽ ζ2 -> ζ2 ≽ ζ3 -> ζ1 ≽ ζ3.
+  Proof.
+    intros [ζ12 H12] [ζ23 H23]. rewrite H23, H12.
+    exists (ζ12 ⊙ˢ ζ23). apply Sub.comp_assoc.
+  Qed.
+
+  Lemma geq_precom {w0 w1 w2 w3} (ζ1 : w0 ⊒ˢ w1) (ζ2 : w1 ⊒ˢ w2) (ζ3 : w1 ⊒ˢ w3) :
+    ζ2 ≽ ζ3 -> ζ1 ⊙ˢ ζ2 ≽ ζ1 ⊙ˢ ζ3.
+  Proof. intros [ζ23 ->]. exists ζ23. symmetry. apply Sub.comp_assoc. Qed.
+
+  Lemma geq_max {w1 w2} (ζ : w1 ⊒ˢ w2) : id ≽ ζ.
+  Proof. exists ζ. symmetry. apply Sub.comp_id_left. Qed.
+
+  Lemma geq_extend {w0 w1 w2} (ζ1 : w0 ⊒ˢ w1) (ζ2 : w1 ⊒ˢ w2) : ζ1 ≽ ζ1 ⊙ˢ ζ2.
+  Proof. now exists ζ2. Qed.
+
+  Fixpoint geqb {w0 w1} (ζ1 : w0 ⊒⁻ w1) [w2] (ζ2 : w0 ⊒ˢ w2) {struct ζ1} : bool :=
+    match ζ1 with
+    | Tri.refl => true
+    | Tri.cons x t ζ1 =>
+        let ζ2' := thin _ ⊙ˢ ζ2 in
+        if Ty_eqdec (subst (Ty_hole _) ζ2) (subst t ζ2')
+        then geqb ζ1 ζ2'
+        else false
+    end.
+  Infix "≽?" := geqb (at level 80).
+
+  Lemma geqb_spec {w0 w1} (ζ1 : w0 ⊒⁻ w1) :
+    forall [w2] (ζ2 : w0 ⊒ˢ w2),
+      Bool.reflect (triangular ζ1 ≽ ζ2) (ζ1 ≽? ζ2).
+  Proof.
+    induction ζ1; cbn [geqb triangular]; intros w2 ζ2.
+    - constructor. apply geq_max.
+    - destruct Ty_eqdec.
+      + destruct (IHζ1 _ (thin xIn ⊙ˢ ζ2)); constructor; clear IHζ1.
+        * destruct g as [ζ2']. exists ζ2'.
+          rewrite comp_assoc. rewrite <- H. clear - e.
+          apply env.lookup_extensional.
+          intros y yIn.
+          rewrite lookup_comp.
+          rewrite lookup_thick. unfold thickIn.
+          destruct (occurs_check_view xIn yIn). apply e.
+          cbn. rewrite lookup_comp. unfold thin.
+          now rewrite env.lookup_tabulate.
+        * intros [ζ2' ->]. apply n. clear n. exists ζ2'.
+          rewrite <- ?comp_assoc.
+          rewrite comp_thin_thick.
+          rewrite comp_id_left.
+          reflexivity.
+      + constructor. intros [ζ2' ->]. apply n. clear n.
+        rewrite <- ?comp_assoc.
+        rewrite comp_thin_thick.
+        rewrite comp_id_left.
+        cbn. rewrite ?lookup_comp, lookup_thick.
+        unfold thickIn. rewrite occurs_check_view_refl.
+        now rewrite subst_comp.
+  Qed.
+
+End Sub.
+Infix "⊒ˢ" := Sub.Sub.
+Infix "⊙ˢ" := Sub.comp (at level 60, right associativity).
+Infix "≽ˢ" := Sub.geq (at level 80).
+(* Infix "≽?" := Sub.geqb (at level 80). *)
+
+(* Infix "≽⁻" := Tri.geq (at level 80). *)
+(* Infix "≽?" := Sub.geqb (at level 80). *)
 
 Section OccursCheck.
   Import option.notations.
@@ -236,38 +571,60 @@ Section OccursCheck.
     fun w =>
       fix oc (t : Ty w) (y : nat) (yIn : y ∈ w) {struct t} :=
       match t with
-      | t_evar xIn   => Some t_evar <*> occurs_check_in xIn yIn
-      | t_bool       => Some t_bool
-      | t_func T1 T2 => Some t_func <*> oc T1 y yIn <*> oc T2 y yIn
+      | Ty_hole xIn   => Some Ty_hole <*> occurs_check_in xIn yIn
+      | Ty_bool       => Some Ty_bool
+      | Ty_func T1 T2 => Some Ty_func <*> oc T1 y yIn <*> oc T2 y yIn
       end.
 
-  Lemma occurs_check_thin {Σ x} (xIn : x ∈ Σ) (t : Ty (Σ - x)) :
+  Lemma occurs_check_thin {w x} (xIn : x ∈ w) (t : Ty (w - x)) :
     option.wp (eq t) (occurs_check (thin xIn t) xIn).
   Proof.
     induction t; cbn.
-    - rewrite option.wp_map. unfold occurs_check_in.
-      rewrite occurs_check_view_thin. now constructor.
     - now constructor.
     - repeat rewrite ?option.wp_aplazy, ?option.wp_map.
       repeat option.tactics.mixin. congruence.
+    - rewrite option.wp_map. unfold occurs_check_in.
+      rewrite occurs_check_view_thin. now constructor.
   Qed.
 
-  Lemma occurs_check_sound {Σ} (t : Ty Σ) {x} (xIn : x ∈ Σ) :
+  Lemma occurs_check_sound {w} (t : Ty w) {x} (xIn : x ∈ w) :
     option.wlp (fun t' => t = thin xIn t') (occurs_check t xIn).
   Proof.
     induction t; cbn.
-    - unfold occurs_check_in.
-      now destruct occurs_check_view; constructor.
     - now constructor.
     - repeat rewrite ?option.wlp_aplazy, ?option.wlp_map.
       repeat option.tactics.mixin. cbn. congruence.
+    - unfold occurs_check_in.
+      now destruct occurs_check_view; constructor.
+  Qed.
+
+  Lemma occurs_check_spec {w x} (xIn : x ∈ w) (t : Ty w) :
+    option.spec
+      (fun t' => t = thin xIn t')
+      (t = Ty_hole xIn \/ Ty_subterm (Ty_hole xIn) t)
+      (occurs_check t xIn).
+  Proof.
+    induction t; cbn.
+    - constructor. reflexivity.
+    - repeat option.tactics.mixin; subst; auto; right;
+        match goal with
+        | H: _ \/ Ty_subterm _ ?t |- _ =>
+            destruct H;
+            [ subst; constructor; constructor
+            | constructor 2 with t; auto; constructor; constructor
+            ]
+        end.
+    - unfold occurs_check_in.
+      destruct (occurs_check_view xIn i0); constructor.
+      + left. reflexivity.
+      + reflexivity.
   Qed.
 
 End OccursCheck.
 
 Definition box_intro_split {A} :
   ⊢ A -> ►□A -> □A :=
-  fun Σ0 a la Σ1 ζ =>
+  fun w0 a la w1 ζ =>
     match ζ with
     | Tri.refl => a
     | Tri.cons x t ζ' => la x _ t _ ζ'
@@ -276,32 +633,32 @@ Definition box_intro_split {A} :
 Definition SUBST : TYPE := Ty -> □Ty.
 Section Subst.
 
-  Context [Σ] (lsubst : ▻(Ty -> □Ty) Σ).
+  Context [w] (lsubst : ▻(Ty -> □Ty) w).
 
-  Definition subst_in {x} (xIn : In x Σ) : □Ty Σ :=
+  Definition subst_in {x} (xIn : In x w) : □Ty w :=
     box_intro_split
-      (t_evar xIn)
+      (Ty_hole xIn)
       (fun y yIn s =>
          match occurs_check_view yIn xIn with
          | Same _     => lsubst yIn s
-         | Diff _ xIn => lsubst yIn (t_evar xIn)
+         | Diff _ xIn => lsubst yIn (Ty_hole xIn)
          end).
 
-  Definition subst : Ty Σ -> □Ty Σ :=
-    fix subst (t : Ty Σ) : □Ty Σ :=
+  Definition subst : Ty w -> □Ty w :=
+    fix subst (t : Ty w) : □Ty w :=
       match t with
-      | t_evar xIn   => subst_in xIn
-      | t_bool       => fun _ _ => t_bool
-      | t_func T1 T2 => fun _ ζ => t_func (subst T1 _ ζ) (subst T2 _ ζ)
+      | Ty_hole xIn   => subst_in xIn
+      | Ty_bool       => fun _ _ => Ty_bool
+      | Ty_func T1 T2 => fun _ ζ => Ty_func (subst T1 _ ζ) (subst T2 _ ζ)
       end.
 
 End Subst.
 
-Definition realsubst_fast : ⊢ Ty -> □Ty :=
-  Löb SUBST subst.
+(* Definition realsubst_fast : ⊢ Ty -> □Ty := *)
+(*   Löb SUBST subst. *)
 
 Definition realsubst_slow : ⊢ Ty -> □Ty.
-  refine (fix subst {Σ} (t : Ty Σ) {Σ1} ζ1 {struct ζ1} := _).
+  refine (fix subst {w} (t : Ty w) {w1} ζ1 {struct ζ1} := _).
   destruct ζ1.
   - apply t.
   - refine (subst _ _ _ ζ1).
@@ -313,32 +670,32 @@ Definition Hom (A B : TYPE) := ⊢ A -> B.
 
 Definition fmap {A B} (f : Hom A B) : Hom ◆A ◆B.
 Proof.
-  intros Σ0 [[Σ1 [ζ1 a1]]|].
-  - constructor 1. exists Σ1. split. auto. apply f. auto.
+  intros w0 [[w1 [ζ1 a1]]|].
+  - constructor 1. exists w1. split. auto. apply f. auto.
   - constructor 2.
 Defined.
 (* Notation "f <$> a" := (fmap f a) (at level 20). *)
 
+Local Notation "s [ ζ ]" :=
+  (Sub.subst s ζ)
+    (at level 8, left associativity,
+      format "s [ ζ ]").
+Local Coercion Sub.triangular : Tri.Tri >-> Sub.Sub.
+
 Section Mult.
   Import option.notations.
 
+  Definition acc {A} {w0 w1} (ζ1 : w0 ⊒⁻ w1) : ◆A w1 -> ◆A w0 :=
+    option.map (fun '(existT _ w2 (ζ2 , a)) => existT _ w2 (ζ1 ⊙ ζ2, a)).
+
   Definition μ {A} : Hom ◆◆A ◆A :=
-    fun Σ0 a0 =>
-      '(Σ1; (ζ1 , a1)) <- a0;;
-      '(Σ2; (ζ2 , a2)) <- a1;;
-      Some (Σ2; (Tri.trans ζ1 ζ2, a2)).
+    fun w0 a0 => '(w1; (ζ1 , a1)) <- a0;; acc ζ1 a1.
 
   Definition ebind {A B} : Hom A ◆B -> Hom ◆A ◆B :=
-    fun f Σ0 a0 =>
-      '(Σ1; (ζ1, a1)) <- a0 ;;
-      '(Σ2; (ζ2, b2)) <- f Σ1 a1 ;;
-      Some (Σ2; (Tri.trans ζ1 ζ2, b2)).
+    fun f w0 a0 => '(w1; (ζ1, a1)) <- a0 ;; acc ζ1 (f w1 a1).
 
   Definition bind {A B} : ⊢ ◆A -> □(A -> ◆B) -> ◆B :=
-    fun Σ a0 f =>
-      '(Σ1; (ζ1 , a1)) <- a0 ;;
-      '(Σ2; (ζ2 , b2)) <- f Σ1 ζ1 a1 ;;
-      Some (Σ2; (Tri.trans ζ1 ζ2, b2)).
+    fun w a0 f => '(w1; (ζ1 , a1)) <- a0 ;; acc ζ1 (f w1 ζ1 a1).
 
 End Mult.
 
@@ -350,70 +707,277 @@ Notation "⟨ ζ ⟩ x <- ma ;; mb" :=
 
 (* see Kobayashi, S. (1997). Monad as modality. *)
 Definition strength {A B} : Hom (□A * ◆B) (◆(□A * B)) :=
-  fun Σ0 '(a0,b0) => bind b0 (fun Σ1 ζ1 b1 => η (four a0 ζ1, b1)).
+  fun w0 '(a0,b0) => bind b0 (fun w1 ζ1 b1 => η (four a0 ζ1, b1)).
 
-Definition Assignment : TYPE :=
-  @Env nat (fun _ => Ty ctx.nil).
-Definition Lift (A : Type) : TYPE :=
-  fun Σ => (Assignment Σ -> A)%type.
+(* Definition Lift (A : Type) : TYPE := *)
+(*   fun w => (Assignment w -> A)%type. *)
 Definition Const (A : Type) : TYPE :=
   fun _ => A.
 Definition PROP : TYPE :=
   fun _ => Prop.
 
+(* Notation "ζ1 ≽ ζ2" := (Subgeq ζ1 ζ2) (at level 80). *)
+(* Notation "ζ1 ≲ ζ2" := (Subleq ζ1 ζ2) (at level 80). *)
+(* Notation "ζ1 ≼ ζ2" := (Trileq ζ1 ζ2) (at level 80). *)
+
 Definition Property : TYPE :=
-  □PROP.
+  fun w => forall w', w ⊒ˢ w' -> Prop.
+  (* □PROP. *)
 
-Definition Unifies : ⊢ Ty -> Ty -> Property.
-  intros Σ s t Σ1 ζ1.
-  apply (realsubst_slow s ζ1 = realsubst_slow t ζ1).
-Defined.
+Module P.
 
-Notation "ζ ⊨ s ~ t" := (Unifies s t ζ) (at level 90, s at level 69).
+  Section Instances.
+
+    Context {w : World}.
+
+    Definition iff (P Q : Property w) : Prop :=
+      forall Δ ζ, P Δ ζ <-> Q Δ ζ.
+    Infix "<->" := iff.
+
+    Instance iff_refl : Reflexive iff.
+    Proof. unfold Reflexive, iff. intros. reflexivity. Qed.
+    Instance iff_sym : Symmetric iff.
+    Proof. unfold Symmetric, iff. intros. now symmetry. Qed.
+    Instance iff_trans : Transitive iff.
+    Proof. unfold Transitive, iff. intros. now transitivity (y Δ ζ). Qed.
+
+    Instance iff_equiv : Equivalence iff.
+    Proof. constructor; auto with typeclass_instances. Qed.
+
+    Definition and (P Q : Property w) : Property w :=
+      fun _ ζ => P _ ζ /\ Q _ ζ.
+    Instance proper_and : Proper (iff ==> iff ==> iff) and.
+    Proof. firstorder. Qed.
+
+    Definition impl (P Q : Property w) : Property w :=
+      (fun w' ζ => P w' ζ -> Q w' ζ)%type.
+
+    Definition nothing (P : Property w) : Prop :=
+      forall w' ζ, P w' ζ -> False.
+    Instance proper_nothing : Proper (iff ==> Logic.iff) nothing.
+    Proof. intros ? ? ?. do 2 (apply forall_proper; intros ?). intuition. Qed.
+
+    Definition max (P : Property w) : Property w :=
+      and P (fun w1 ζ1 => forall w2 ζ2, P w2 ζ2 -> ζ1 ≽ˢ ζ2).
+    Instance proper_max : Proper (iff ==> iff) max.
+    Proof. firstorder. Qed.
+    Instance proper_max' : Proper (iff ==> forall_relation (fun w => eq ==> Basics.flip Basics.impl)) max.
+    Proof. repeat intro; subst; firstorder. Qed.
+
+  End Instances.
+  #[export] Existing Instance iff_refl.
+  #[export] Existing Instance iff_sym.
+  #[export] Existing Instance iff_trans.
+  #[export] Existing Instance iff_equiv.
+  #[export] Existing Instance proper_and.
+  #[export] Existing Instance proper_nothing.
+  #[export] Existing Instance proper_max.
+  #[export] Existing Instance proper_max'.
+
+
+  Notation "P <-> Q" := (iff P Q).
+
+  Definition unifies : ⊢ Ty -> Ty -> Property :=
+    fun w s t w1 (ζ1 : w ⊒ˢ w1) => s[ζ1] = t[ζ1].
+
+  Definition unifiesX : ⊢ Ty -> Ty -> Property :=
+    fun w0 s t =>
+      match s , t with
+      | Ty_hole xIn as s , t               => unifies s t
+      | s               , Ty_hole yIn as t => unifies s t
+      | Ty_bool          , Ty_bool          => fun _ _ => True
+      | Ty_func s1 s2    , Ty_func t1 t2    => and (unifies s1 t1) (unifies s2 t2)
+      | s               , t               => fun _ _ => False
+      end.
+
+  Definition unifiesY : ⊢ Ty -> Ty -> Property :=
+    fun w0 =>
+      fix ufs s t {struct s} :=
+      match s , t with
+      | Ty_hole xIn as s , t               => unifies s t
+      | s               , Ty_hole yIn as t => unifies s t
+      | Ty_bool          , Ty_bool          => fun _ _ => True
+      | Ty_func s1 s2    , Ty_func t1 t2    => and (ufs s1 t1) (ufs s2 t2)
+      | _               , _               => fun _ _ => False
+      end.
+
+  Lemma unifies_sym {w} (s t : Ty w) : iff (unifies s t) (unifies t s).
+  Proof. now unfold iff, unifies. Qed.
+
+  Lemma unifiesX_equiv {w} (s t : Ty w) : iff (unifies s t) (unifiesX s t).
+  Proof.
+    destruct s; cbn; [| |reflexivity]; try now destruct t.
+    destruct t; auto.
+    - split; intuition discriminate.
+    - unfold iff, unifies, and; cbn. intuition congruence.
+    - reflexivity.
+  Qed.
+
+  Lemma unifiesY_equiv {w} (s t : Ty w) : iff (unifies s t) (unifiesY s t).
+  Proof.
+    revert t; induction s; intros t; destruct t; cbn in *;
+      try reflexivity;
+      try (unfold iff, unifies; cbn; intuition congruence).
+    - rewrite <- IHs1, <- IHs2.
+      unfold iff, unifies, and; cbn.
+      intuition congruence.
+  Qed.
+
+  Definition DClosed {w} (P : Property w) : Prop :=
+    forall w1 w2 (ζ1 : w ⊒ˢ w1) (ζ2 : w ⊒ˢ w2),
+      ζ1 ≽ˢ ζ2 -> P w1 ζ1 -> P w2 ζ2.
+
+  Lemma dclosed_unifies {w} (s t : Ty w) : DClosed (P.unifies s t).
+  Proof.
+    unfold DClosed, P.unifies.
+    intros ? ? ? ? [? ->] ?.
+    Set Printing Coercions.
+    rewrite ?Sub.subst_comp.
+    now f_equal.
+  Qed.
+
+  Definition extend {w1 w2} (P : Property w1) (ζ1 : w1 ⊒ˢ w2) : Property w2 :=
+    fun Δ ζ2 => P Δ (ζ1 ⊙ˢ ζ2).
+
+  Lemma extend_id {w0} (P : Property w0) :
+    iff (extend P Sub.id) P.
+  Proof.
+    unfold iff, extend. intros.
+    now rewrite Sub.comp_id_left.
+  Qed.
+
+  Lemma extend_and {w0 w1} (P Q : Property w0) (ζ1 : w0 ⊒⁻ w1) :
+    iff (extend (and P Q) ζ1) (and (extend P ζ1) (extend Q ζ1)).
+  Proof. reflexivity. Qed.
+
+  Lemma extend_unifies {w0 w1} (s t : Ty w0) (ζ : w0 ⊒⁻ w1) :
+    iff (unifies s[ζ] t[ζ]) (extend (unifies s t) ζ).
+  Proof.
+    unfold iff, extend, unifies. intros.
+    now rewrite ?Sub.subst_comp.
+  Qed.
+
+  Lemma optimists {w0 w1 w2 w3} (P Q : Property w0) (ζ1 : w0 ⊒ˢ w1) (ζ2 : w1 ⊒ˢ w2) (ζ3 : w2 ⊒ˢ w3) :
+    DClosed P ->
+    max (extend P ζ1) ζ2 ->
+    max (extend Q (ζ1 ⊙ˢ ζ2)) ζ3 ->
+    max (extend (and P Q) ζ1) (ζ2 ⊙ˢ ζ3).
+  Proof.
+    unfold DClosed, extend.
+    intros dcp [p12 pmax] [q123 qmax].
+    split.
+    split.
+    - revert p12. apply dcp.
+      apply Sub.geq_precom.
+      apply Sub.geq_extend.
+    - revert q123. now rewrite Sub.comp_assoc.
+    - intros ? f [H1 H2].
+      apply pmax in H1.
+      destruct H1 as [g ?].
+      subst f.
+      apply Sub.geq_precom.
+      apply qmax.
+      now rewrite Sub.comp_assoc.
+  Qed.
+
+  Lemma optimists_unifies {w w1 w2 w3} {s1 s2 t1 t2 : Ty w}
+    (ζ1 : w ⊒ˢ w1) (ζ2 : w1 ⊒ˢ w2) (ζ3 : w2 ⊒ˢ w3) :
+    max (unifies s1[ζ1] t1[ζ1]) ζ2 ->
+    max (unifies s2[ζ1 ⊙ˢ ζ2] t2[ζ1 ⊙ˢ ζ2]) ζ3 ->
+    max (and (unifies s1[ζ1] t1[ζ1]) (unifies s2[ζ1] t2[ζ1])) (ζ2 ⊙ˢ ζ3).
+  Proof.
+    unfold max, and, unifies. rewrite ?Sub.subst_comp.
+    intros [p12 pmax] [q123 qmax]. split. split; congruence.
+    intros w4 ζ4 [H1 H2].
+    apply pmax in H1. destruct H1 as [ζ24 ->]. rewrite ?Sub.subst_comp in H2.
+    apply qmax in H2. destruct H2 as [ζ34 ->].
+    apply Sub.geq_precom.
+    apply Sub.geq_extend.
+  Qed.
+
+End P.
+
+(* Notation "ζ ⊨ s ~ t" := (Unifies s t ζ) (at level 90, s at level 69). *)
+
+(* Fixpoint models' {w1 w2} (ι : Assignment w1) (ζ : w1 ⊒⁻ w2) : Prop := *)
+(*   match ζ with *)
+(*   | Tri.refl       => True *)
+(*   | Tri.cons x t ζ => *)
+(*       let ι' := env.remove _ ι _ in *)
+(*       env.lookup ι _ = Sub.subst t ι' /\ models' ι' ζ *)
+(*   end. *)
+
+(* Definition models {w1 w2} (ι1 : Assignment w1) (ζ : w1 ⊒⁻ w2) : Prop. *)
+(*   refine (exists (ι2 : Assignment w2), ι1 = _). *)
+(*   apply env.tabulate. *)
+(*   intros x xIn. *)
+(*   refine (Sub.subst _ ι2). *)
+(*   refine (realsubst_slow (Ty_hole xIn) ζ). *)
+(* Defined. *)
 
 Definition wp {A} : ⊢ ◆A -> □(A -> PROP) -> PROP :=
-  fun Σ0 a0 POST => option.wp (fun '(Σ1; (ζ1 , a1)) => POST Σ1 ζ1 a1) a0.
+  fun w0 a0 POST => option.wp (fun '(w1; (ζ1 , a1)) => POST w1 ζ1 a1) a0.
 
 Definition wlp {A} : ⊢ ◆A -> □(A -> PROP) -> PROP :=
-  fun Σ0 a0 POST => option.wlp (fun '(Σ1; (ζ1 , a1)) => POST Σ1 ζ1 a1) a0.
+  fun w0 a0 POST => option.wlp (fun '(w1; (ζ1 , a1)) => POST w1 ζ1 a1) a0.
 
-Lemma wp_η {A Σ} (a : A Σ) (POST : □(A -> PROP) Σ) :
+Definition spec {A} : ⊢ ◆A -> □(A -> PROP) -> PROP -> PROP :=
+  fun w0 a0 SPOST NPOST => option.spec (fun '(w1; (ζ1 , a1)) => SPOST w1 ζ1 a1) NPOST a0.
+
+Lemma wp_η {A w} (a : A w) (POST : □(A -> PROP) w) :
   wp (η a) POST <-> T POST a.
 Proof. unfold wp, η. now option.tactics.mixin. Qed.
 
-Lemma wp_μ {A B Σ} (a : ◆A Σ) (f : □(A -> ◆B) Σ) (POST : □(B -> PROP) Σ) :
+Lemma wp_μ {A B w} (a : ◆A w) (f : □(A -> ◆B) w) (POST : □(B -> PROP) w) :
   wp (bind a f) POST <-> wp a (fun _ ζ1 a1 => wp (f _ ζ1 a1) (four POST ζ1)).
 Proof.
-  unfold wp, bind.
+  unfold wp, bind, acc.
   now repeat
-    (rewrite ?option.wp_bind;
+    (rewrite ?option.wp_bind, ?option.wp_map;
      repeat option.tactics.mixin;
      intros; try destruct_conjs).
 Qed.
 
-Lemma wlp_η {A Σ} (a : A Σ) (POST : □(A -> PROP) Σ) :
+Lemma wlp_η {A w} (a : A w) (POST : □(A -> PROP) w) :
   wlp (η a) POST <-> T POST a.
 Proof. unfold wlp, η. now option.tactics.mixin. Qed.
 
-Lemma wlp_μ {A B Σ} (a : ◆A Σ) (f : □(A -> ◆B) Σ) (POST : □(B -> PROP) Σ) :
+Lemma wlp_μ {A B w} (a : ◆A w) (f : □(A -> ◆B) w) (POST : □(B -> PROP) w) :
   wlp (bind a f) POST <-> wlp a (fun _ ζ1 a1 => wlp (f _ ζ1 a1) (four POST ζ1)).
 Proof.
-  unfold wlp, bind.
+  unfold wlp, bind, acc.
   now repeat
-    (rewrite ?option.wlp_bind;
+    (rewrite ?option.wlp_bind, ?option.wlp_map;
      repeat option.tactics.mixin;
      intros; try destruct_conjs).
+Qed.
+
+Lemma spec_η {A w} (a : A w) (SPOST : □(A -> PROP) w) (NPOST : PROP w) :
+  spec (η a) SPOST NPOST <-> T SPOST a.
+Proof.
+  unfold spec, η. now option.tactics.mixin.
+Qed.
+
+Lemma spec_μ {A B w} (a : ◆A w) (f : □(A -> ◆B) w) (SPOST : □(B -> PROP) w) (NPOST : PROP w) :
+  spec (bind a f) SPOST NPOST <->
+  spec a (fun _ ζ1 a1 => spec (f _ ζ1 a1) (four SPOST ζ1) NPOST) NPOST.
+Proof.
+  unfold spec, bind, acc.
+  repeat
+    (rewrite ?option.spec_bind, ?option.spec_map;
+     repeat option.tactics.mixin;
+     intros; try destruct_conjs); try reflexivity.
 Qed.
 
 Section VarView.
 
-  Inductive VarView {Σ} : Ty Σ -> Type :=
-  | is_var {x} (xIn : x ∈ Σ) : VarView (t_evar xIn)
-  | not_var {t} (H: forall x (xIn : x ∈ Σ), t <> t_evar xIn) : VarView t.
+  Inductive VarView {w} : Ty w -> Type :=
+  | is_var {x} (xIn : x ∈ w) : VarView (Ty_hole xIn)
+  | not_var {t} (H: forall x (xIn : x ∈ w), t <> Ty_hole xIn) : VarView t.
 
-  Definition varview {Σ} (t : Ty Σ) : VarView t :=
+  Definition varview {w} (t : Ty w) : VarView t :=
     match t with
-    | t_evar xIn => is_var xIn
+    | Ty_hole xIn => is_var xIn
     | _ => ltac:(constructor 2; discriminate)
     end.
 
@@ -423,38 +987,93 @@ Section VarView.
   (*   Eval cbv [varview] in @varview. *)
   (* Next Obligation *)
   (* | tf_bool *)
-  (* | tf_func (T1 T2 : T Σ). *)
+  (* | tf_func (T1 T2 : T w). *)
   (* Global Arguments tf_bool {_ _}. *)
   (* Global Arguments tf_func {_ _} T1 T2. *)
 
   (* Definition Var : TYPE := *)
-  (*   fun Σ => {x & In x Σ}. *)
+  (*   fun w => {x & In x w}. *)
 
   (* Definition unfold : ⊢ Ty -> Sum Var (TyF Ty) := *)
-  (*   fun Σ t => match t with *)
-  (*              | t_evar xIn   => inl (_;xIn) *)
-  (*              | t_bool       => inr (tf_bool) *)
-  (*              | t_func t1 t2 => inr (tf_func t1 t2) *)
+  (*   fun w t => match t with *)
+  (*              | Ty_hole xIn   => inl (_;xIn) *)
+  (*              | Ty_bool       => inr (tf_bool) *)
+  (*              | Ty_func t1 t2 => inr (tf_func t1 t2) *)
   (*              end. *)
 
   (* Definition fold : ⊢ Sum Var (TyF Ty) -> Ty := *)
-  (*   fun Σ t => match t with *)
-  (*              | inl (_;xIn) => t_evar xIn *)
-  (*              | inr (tf_bool) => t_bool *)
-  (*              | inr (tf_func t1 t2) => t_func t1 t2 *)
+  (*   fun w t => match t with *)
+  (*              | inl (_;xIn) => Ty_hole xIn *)
+  (*              | inr (tf_bool) => Ty_bool *)
+  (*              | inr (tf_func t1 t2) => Ty_func t1 t2 *)
   (*              end. *)
 
 End VarView.
 
+Lemma trivialproblem {w} (t : Ty w) :
+  P.max (P.unifies t t) Sub.id.
+Proof.
+  unfold P.max. split.
+  - reflexivity.
+  - intros ? ζ ?. exists ζ.
+    now rewrite Sub.comp_id_left.
+Qed.
+
+Lemma varelim {w x} (xIn : x ∈ w) (t : Ty (w - x)) :
+  P.max (P.unifies (Ty_hole xIn) (thin xIn t)) (Sub.thick xIn t).
+Proof.
+  rewrite Sub.subst_thin.
+  split.
+  - unfold P.unifies. cbn.
+    rewrite Sub.lookup_thick.
+    unfold thickIn.
+    rewrite occurs_check_view_refl.
+    rewrite <- Sub.subst_comp.
+    rewrite Sub.comp_thin_thick.
+    rewrite Sub.subst_id.
+    reflexivity.
+  - unfold P.unifies, Sub.geq. cbn. intros * Heq.
+    exists (Sub.comp (Sub.thin xIn) ζ2).
+    apply env.lookup_extensional. intros y yIn.
+    rewrite ?Sub.lookup_comp.
+    rewrite Sub.lookup_thick.
+    rewrite Sub.subst_comp.
+    unfold thickIn.
+    destruct (occurs_check_view xIn yIn); cbn.
+    + apply Heq.
+    + now rewrite Sub.lookup_thin.
+Qed.
+
+Lemma no_cycle {w} (t : Ty w) : ~ Ty_subterm t t.
+Proof. induction (wellfounded (R:=@Ty_subterm w) t). intuition. Qed.
+
+Lemma Ty_subterm_subst {w1 w2} (s t : Ty w1) (ζ : Sub.Sub w1 w2) :
+  Ty_subterm s t -> Ty_subterm (Sub.subst s ζ) (Sub.subst t ζ).
+Proof.
+  unfold Ty_subterm. induction 1; cbn.
+  - constructor 1; destruct H; constructor.
+  - econstructor 2; eauto.
+Qed.
+
+Lemma nothing_unifies_occurs_strictly {w x} (xIn : x ∈ w) (t : Ty w) :
+  Ty_subterm (Ty_hole xIn) t ->
+  P.nothing (P.unifies (Ty_hole xIn) t).
+Proof.
+  unfold P.nothing, P.unifies; intros.
+  apply no_cycle with (Sub.subst t ζ).
+  rewrite <- H0 at 1.
+  now apply Ty_subterm_subst.
+Qed.
+
 Module Variant1.
 
   Definition flex : ⊢ Ty -> ∀ x, In x -> ◆Unit :=
-    fun Σ t x xIn =>
+    fun w t x xIn =>
       match varview t with
       | is_var yIn =>
           match occurs_check_view xIn yIn with
           | Same _      => η tt
-          | Diff _ yIn' => Some (sooner2diamond (_; (xIn; (t_evar yIn', tt))))
+          | Diff _ yIn' => Some (sooner2diamond (_; (xIn; (Ty_hole yIn', tt))))
           end
       | not_var _ =>
           option_map
@@ -462,56 +1081,484 @@ Module Variant1.
             (occurs_check t xIn)
       end.
 
-  Import option.notations.
-  Set Equations With UIP.
-  Lemma flex_sound {Σ y} (t : Ty Σ) (yIn : In y Σ) :
-    wlp (flex t yIn) (fun _ ζ1 _ => ζ1 ⊨ t ~ t_evar yIn).
+
+  Lemma flex_sound {w y} (t : Ty w) (yIn : y ∈ w) :
+    wlp (flex t yIn) (fun _ ζ1 _ => P.unifies t (Ty_hole yIn) ζ1).
   Proof.
-    unfold Unifies, flex, wlp.
+    unfold P.unifies, flex, wlp.
     destruct (varview t).
-    - destruct (occurs_check_view yIn xIn); cbn.
+    - destruct (occurs_check_view yIn xIn).
       + constructor. reflexivity.
-      + constructor; cbn.
+      + constructor. cbn - [Sub.subst].
+        rewrite Sub.comp_id_right. cbn.
+        rewrite ?Sub.lookup_thick. unfold thickIn.
         now rewrite ?occurs_check_view_refl, ?occurs_check_view_thin.
     - repeat rewrite ?option.wlp_aplazy, ?option.wlp_map.
-      generalize (occurs_check_sound t yIn). apply option.wlp_monotonic.
-      intros t' ->; cbn. rewrite occurs_check_view_refl.
-      apply thin_thick.
+      generalize (occurs_check_sound t yIn).
+      apply option.wlp_monotonic.
+      intros t' ->. cbn.
+      rewrite Sub.comp_id_right.
+      rewrite Sub.subst_thin.
+      rewrite <- Sub.subst_comp.
+      rewrite Sub.comp_thin_thick.
+      rewrite Sub.subst_id.
+      rewrite Sub.lookup_thick.
+      unfold thickIn.
+      now rewrite occurs_check_view_refl.
   Qed.
+
+  Lemma flex_complete {w0 w1 y} (ζ1 : w0 ⊒⁻ w1) (t : Ty w0) (yIn : y ∈ w0) :
+    P.unifies t (Ty_hole yIn) ζ1 ->
+    wp (flex t yIn) (fun mgw mgζ _ => mgζ ≽ˢ ζ1).
+  Proof.
+    intros. unfold flex.
+    destruct (varview t).
+    - destruct (occurs_check_view yIn xIn).
+      + constructor. apply Sub.geq_max.
+      + constructor; cbn.
+        rewrite Sub.comp_id_right.
+        apply (@varelim _ _ yIn).
+        now symmetry.
+    - unfold wp. apply option.wp_map.
+      destruct (occurs_check_spec yIn t).
+      + constructor. cbn. subst.
+        rewrite Sub.comp_id_right.
+        apply varelim. now symmetry.
+      + exfalso. destruct H1.
+        * specialize (H0 _ yIn). contradiction.
+        * apply nothing_unifies_occurs_strictly in H1.
+          now apply (H1 _ ζ1).
+  Qed.
+
+  Lemma flex_spec {w x} (xIn : x ∈ w) (t : Ty w) :
+    let P := P.unifies (Ty_hole xIn) t in
+    spec
+      (flex t xIn)
+      (fun w' ζ' _ => P.max P ζ')
+      (P.nothing P).
+  Proof.
+    unfold flex.
+    destruct (varview t).
+    - destruct (occurs_check_view xIn xIn0); subst.
+      + constructor. apply trivialproblem.
+      + constructor. cbn.
+        rewrite Sub.comp_id_right.
+        change (Ty_hole (in_thin xIn yIn)) with (thin xIn (Ty_hole yIn)).
+        apply varelim.
+    - unfold spec. rewrite option.spec_map.
+      generalize (occurs_check_spec xIn t).
+      apply option.spec_monotonic.
+      + intros t' ->. cbn.
+        rewrite Sub.comp_id_right.
+        apply varelim.
+      + specialize (H _ xIn).
+        intros []. contradiction.
+        now apply nothing_unifies_occurs_strictly.
+  Qed.
+
+  Definition spec' {A} : ⊢ ◆A -> □(Option A -> PROP) -> PROP.
+    refine (fun w0 a0 POST => _).
+    destruct a0 as [[w1 [ζ1 a]]|].
+    cbv. apply (POST w1 ζ1 (Some a)).
+    apply (POST w0 Tri.refl None).
+  Defined.
+
+  Definition Wpure : TYPE -> TYPE :=
+    fun A => □(A -> PROP) -> PROP.
+  Definition DiamondT (M : TYPE -> TYPE) : TYPE -> TYPE :=
+    fun A => M (fun w0 => {w1 : World & ((w0 ⊒⁻ w1) * A w1)}%type).
+  Definition OptionT (M : TYPE -> TYPE) : TYPE -> TYPE :=
+    fun A => M (Option A).
+
+  Definition W := DiamondT (OptionT Wpure).
+
+  Definition flexspecw : ⊢ Ty -> ∀ x, In x -> W Unit.
+  Proof.
+    cbv [Impl Valid Box Forall PROP W OptionT DiamondT Wpure Option].
+    intros w0 t x xIn POST.
+    refine (exists w1 : World, exists ζ1 : w0 ⊒⁻ w1, POST w1 ζ1 _).
+    destruct (eq_dec (Ty_hole xIn)[ζ1] t[ζ1]).
+    apply Some. exists w1. split. apply Tri.refl. apply tt.
+    apply None.
+  Defined.
+
+  Definition flexspec : ⊢ Ty -> ∀ x, In x -> □(Option Unit -> PROP) -> PROP.
+  Proof.
+    cbv [Impl Valid Box Forall PROP].
+    intros w0 t x xIn POST.
+    refine (exists w1 : World, exists ζ1 : w0 ⊒⁻ w1, POST w1 ζ1 _).
+    destruct (eq_dec (Ty_hole xIn)[ζ1] t[ζ1]).
+    apply (Some tt).
+    apply None.
+  Defined.
+
+  Definition order {Unit} : ⊢ (□(Option Unit -> PROP) -> PROP) -> (□(Option Unit -> PROP) -> PROP) -> PROP :=
+    fun w0 PT QT =>
+      forall (P Q : □(Option Unit -> PROP) w0),
+        (forall w1 (ζ1 : w0 ⊒⁻ w1) (x : Option Unit w1),
+            P w1 ζ1 x -> Q w1 ζ1 x) ->
+        PT P -> QT Q.
+
+  Lemma flexverify {w} (t : Ty w) {x} (xIn : x ∈ w) :
+    order (spec' (flex t xIn)) (flexspec t xIn).
+  Proof.
+    unfold flex. destruct (varview t) as [y yIn|].
+    - destruct (occurs_check_view xIn yIn); unfold order, spec', flexspec, η;
+        cbn - [eq_dec]; intros P Q PQ HP.
+      + exists w. exists Tri.refl. rewrite eq_dec_refl. auto.
+      + exists (w - x). exists (Tri.single x (Ty_hole yIn)).
+  Admitted.
+
+  Definition cflex : ⊢ Ty -> Ty -> Option Unit :=
+    fun w s t => if eq_dec s t then Some tt else None.
+
+  Definition mg : ⊢ ◆Unit -> □(Option Unit -> PROP) :=
+    fun w0 d w1 ζ1 o =>
+      match o , d with
+      | Some _ , Some (existT _ mgw (mgζ , _)) => mgζ ≽ˢ ζ1
+      | None   , _                             => True
+      | Some _ , None                          => False
+      end.
+
+  Module Related.
+    Definition DUM {w0 w1} (ζ1 : w0 ⊒⁻ w1) (spec : Option Unit w1) : Type :=
+      { m : ◆Unit w0 | mg m ζ1 spec }.
+
+    Definition dret {w0 w1} (ζ1 : w0 ⊒⁻ w1) (a : Unit w0) : DUM ζ1 (Some a) :=
+      exist _ (Some (w0; (Tri.refl, a))) (Sub.geq_max ζ1).
+
+    Definition flexspec {w0} (t : Ty w0) {x} (xIn : x ∈ w0) {w1} (ζ1 : w0 ⊒⁻ w1) : Option Unit w1 :=
+      if eq_dec (Ty_hole xIn)[ζ1] t[ζ1] then Some tt else None.
+
+    Program Definition dflex {w0} (t : Ty w0) {x} (xIn : x ∈ w0) {w1} (ζ1 : w0 ⊒⁻ w1) : DUM ζ1 (flexspec t xIn ζ1) :=
+        match varview t with
+        | is_var yIn =>
+            match occurs_check_view xIn yIn with
+            | Same _      => η tt
+            | Diff _ yIn' => Some (sooner2diamond (_; (xIn; (Ty_hole yIn', tt))))
+            end
+        | not_var _ =>
+            option_map
+              (fun t' => sooner2diamond (x; (xIn; (t', tt))))
+              (occurs_check t xIn)
+        end.
+    Admit Obligations.
+
+  End Related.
+
+  (* Module DijkstraM. *)
+  (*   Definition obs {w} (m : ◆Unit w) {w2} (ζ2 : w ⊒ˢ w2) : Option Unit w2 := *)
+  (*     match m with *)
+  (*     | Some (x; (ζ1, a)) => if ζ1 ≽? ζ2 then Some a else None *)
+  (*     | None              => None *)
+  (*     end. *)
+
+  (*   Definition DUM {w0 w1} (ζ1 : w0 ⊒⁻ w1) (spec : Option Unit w1) : Type := *)
+  (*     { m : ◆Unit w0 | obs m ζ1 = spec }. *)
+
+  (*   Definition dret {w0 w1} (ζ1 : w0 ⊒⁻ w1) (a : Unit w0) : DUM ζ1 (Some a) := *)
+  (*     exist _ (Some (w0; (Tri.refl, a))) eq_refl. *)
+  (* End DijkstraM. *)
+
+  (* Lemma mg_bind {w0} (da : ◆Unit w0) (dk : □(Unit -> ◆Unit) w0) *)
+  (*   {w1} (ζ1 : w0 ⊒⁻ w1) (oa : Option Unit w1) (ok : Unit w1 -> Option Unit w1) : *)
+  (*   mg da ζ1 oa -> *)
+  (*   (forall {w2} (ζ2 : w ⊒⁻ w2), ζ2 ≽ˢ ζ1 -> mg (dk w1 ζ1 tt) (ok tt) ζ2) -> *)
+  (*   mg (bind da dk) ζ2 (option.bind oa ok). *)
+  (* Proof. *)
+  (*   unfold bind, option.bind, mg at 1. intros mga mgk. *)
+  (*   destruct da as [[? []]|], oa; try easy. *)
+  (*   destruct u, u0. now apply mgk. *)
+  (* Qed. *)
+
+  (* Lemma mg_acc {w w1} (ζ1 : w ⊒⁻ w1) (d : ◆Unit w1) (o : Option Unit w) {w2} (ζ2 : w ⊒⁻ w2) : *)
+  (*   (* mg da oa ζ2 -> *) *)
+  (*   (* (forall {w1} (ζ1 : w ⊒⁻ w1), ζ2 ≲ ζ1 -> mg (acc ζ1 (dk w1 ζ1 tt)) (ok tt) ζ2) -> *) *)
+  (*   mg (acc ζ1 d) o ζ2. *)
+  (* Proof. *)
+  (*   destruct o; cbn; auto. *)
+  (*   destruct d as [[? []]|]; cbn. admit. ; try easy. *)
+  (*   destruct u, u0. now apply mgk. *)
+  (* Qed. *)
+
+  Lemma flexcorrect {w} (t : Ty w) {x} (xIn : x ∈ w) {w2} (ζ2 : w ⊒⁻ w2) :
+    mg (flex t xIn) ζ2 (cflex (Ty_hole xIn)[ζ2] t[ζ2]).
+  Proof.
+    unfold cflex, mg. destruct (eq_dec (Ty_hole xIn)[ζ2] t[ζ2]).
+    - unfold flex. destruct (varview t) as [y yIn|].
+      + destruct (occurs_check_view xIn yIn); cbn.
+        * apply Sub.geq_max.
+        * rewrite Sub.comp_id_right. now apply varelim.
+      + destruct (occurs_check_spec xIn t) as [|[]]; cbn.
+        * rewrite Sub.comp_id_right. subst. now apply varelim.
+        * now apply H in H0.
+        * apply nothing_unifies_occurs_strictly in H0.
+          apply (H0 _ _ e).
+    - destruct (flex t xIn) as [[? [? []]]|]; auto.
+  Qed.
+
+  Definition CMGU : TYPE := Ty -> Ty -> □(Option Unit).
+
+  Section CMgu.
+    Import option.notations.
+    (* Context [w] (lcmgu : ▻CMGU w). *)
+
+    Definition cmgu : ⊢ CMGU :=
+      fun w => fix cmgu s t :=
+        match s , t with
+        | Ty_hole xIn as s , t               => fun _ ζ => cflex s[ζ] t[ζ]
+        | s               , Ty_hole yIn as t => fun _ ζ => cflex s[ζ] t[ζ]
+        | Ty_bool          , Ty_bool          => fun _ _ => Some tt
+        | Ty_func s1 s2    , Ty_func t1 t2    => fun _ ζ => 'tt <- cmgu s1 t1 _ ζ ;; 'tt <- cmgu s2 t2 _ ζ ;; Some tt
+        | _               , _               => fun _ _ => None
+        end.
+  End CMgu.
+
+  (* Definition cmgu : ⊢ CMGU. *)
+  (*   intros w. apply Löb. unfold Valid, Impl. intros w1. Check gcmgu. *)
+  (*   fun w s t => T (@Löb _ @gcmgu w s t). *)
 
   Definition Unifier : TYPE :=
     Ty -> Ty -> ◆Unit.
   Definition BoxUnifier : TYPE :=
     Ty -> Ty -> □◆Unit.
 
+  Definition UnifierSpec : ⊢ Unifier -> PROP :=
+    fun w u =>
+      forall t1 t2,
+        let P := P.unifies t1 t2 in
+        spec
+          (u t1 t2)
+          (fun w2 ζ2 _ => P.max P ζ2)
+          (P.nothing P).
+
+  Definition BoxUnifierSpec : ⊢ BoxUnifier -> PROP :=
+    fun w bu =>
+      forall t1 t2 w1 (ζ1 : w ⊒⁻ w1),
+        let P := P.unifies t1[ζ1] t2[ζ1] in
+        spec
+          (bu t1 t2 w1 ζ1)
+          (fun w2 ζ2 _ => P.max P ζ2)
+          (P.nothing P).
+
   Section MguO.
 
-    Context [Σ] (lmgu : ▻BoxUnifier Σ).
+    Context [w] (lmgu : ▻BoxUnifier w).
+    Context (lmgu_spec : forall x (xIn : x ∈ w),
+                BoxUnifierSpec (lmgu xIn)).
 
-    Definition boxflex {x} (xIn : x ∈ Σ) (t : Ty Σ) : □◆Unit Σ :=
-      box_intro_split (flex t xIn) (fun z zIn u => lmgu _ (t_evar xIn)[z↦u] t[z↦u]).
+    Definition boxflex {x} (xIn : x ∈ w) (t : Ty w) : □◆Unit w :=
+      box_intro_split
+        (flex t xIn)
+        (fun z zIn u =>
+           let ζ := Sub.thick zIn u in
+           lmgu _ (Ty_hole xIn)[ζ] t[ζ]).
 
-    Equations boxmgu : BoxUnifier Σ :=
-    | t_evar xIn   | t            := boxflex xIn t;
-    | s            | t_evar yIn   := boxflex yIn s;
-    | t_bool       | t_bool       := fun _ _ => η tt;
-    | t_func s1 s2 | t_func t1 t2 := fun _ ζ1 =>
-                                       ⟨ ζ2 ⟩ _ <- boxmgu s1 t1 ζ1 ;;
-                                       ⟨ ζ3 ⟩ _ <- boxmgu s2 t2 (Tri.trans ζ1 ζ2) ;;
-                                       η tt;
-    | _            | _            := fun _ _ => None.
+    Import P.
+
+    Lemma boxflex_spec {x} (xIn : x ∈ w) (t : Ty w) (w1 : World) (ζ1 : w ⊒⁻ w1) :
+      let P := P.unifies (Ty_hole xIn)[ζ1] t[ζ1] in
+      spec (boxflex xIn t ζ1) (fun w2 ζ2 _ => P.max P ζ2) (P.nothing P).
+    Proof.
+      destruct ζ1; cbn - [Sub.subst].
+      - rewrite ?Sub.subst_id. apply flex_spec.
+      - rewrite ?Sub.subst_comp. apply lmgu_spec.
+    Qed.
+
+    Definition boxmgu : BoxUnifier w :=
+      fix bmgu s t {struct s} :=
+        match s , t with
+        | Ty_hole xIn   , t            => boxflex xIn t
+        | s            , Ty_hole yIn   => boxflex yIn s
+        | Ty_bool       , Ty_bool       => fun _ _ => η tt
+        | Ty_func s1 s2 , Ty_func t1 t2 =>
+            fun _ ζ1 =>
+              ⟨ ζ2 ⟩ _ <- bmgu s1 t1 _ ζ1 ;;
+              ⟨ ζ3 ⟩ _ <- bmgu s2 t2 _ (Tri.trans ζ1 ζ2) ;;
+              η tt
+        | _            , _            => fun _ _ => None
+        end.
+
+    Section boxmgu_elim.
+
+      Context (P : Ty w -> Ty w -> □◆Unit w -> Type).
+      Context (fflex1 : forall (x : nat) (xIn : x ∈ w) (t : Ty w), P (Ty_hole xIn) t (boxflex xIn t)).
+      Context (fflex2 : forall (x : nat) (xIn : x ∈ w) (t : Ty w), P t (Ty_hole xIn) (boxflex xIn t)).
+      Context (fbool : P Ty_bool Ty_bool (fun (w1 : World) (_ : w ⊒⁻ w1) => η tt)).
+      Context (fbool_func : forall T1 T2 : Ty w, P Ty_bool (Ty_func T1 T2) (fun (w1 : World) (_ : w ⊒⁻ w1) => None)).
+      Context (ffunc_bool : forall T1 T2 : Ty w, P (Ty_func T1 T2) Ty_bool (fun (w1 : World) (_ : w ⊒⁻ w1) => None)).
+      Context (ffunc : forall s1 s2 t1 t2 : Ty w,
+        (P s1 t1 (boxmgu s1 t1)) ->
+        (P s2 t2 (boxmgu s2 t2)) ->
+        P (Ty_func s1 s2) (Ty_func t1 t2)
+          (fun (w1 : World) (ζ1 : w ⊒⁻ w1) =>
+           bind (boxmgu s1 t1 ζ1)
+             (fun (w2 : World) (ζ2 : w1 ⊒⁻ w2) (_ : Unit w2) =>
+              bind (boxmgu s2 t2 (Tri.trans ζ1 ζ2)) (fun (w3 : World) (_ : w2 ⊒⁻ w3) (_ : Unit w3) => η tt)))).
+
+      Lemma boxmgu_elim : forall (t1 t2 : Ty w), P t1 t2 (boxmgu t1 t2).
+      Proof. induction t1; intros t2; cbn; auto; destruct t2; auto. Qed.
+
+    End boxmgu_elim.
+
+    (* Lemma boxmgu_correct (t1 t2 : Ty w) : *)
+    (*   forall {w1} (ζ1 : w ⊒⁻ w1) {w2} (ζ2 : w1 ⊒⁻ w2), *)
+    (*     mg (boxmgu t1 t2 ζ1) (cmgu t1 t2 (ζ1 ⊙ ζ2)) ζ2. *)
+    (* Proof. *)
+    (*   pattern (boxmgu t1 t2). apply boxmgu_elim; clear t1 t2. *)
+    (*   - admit. *)
+    (*   - admit. *)
+    (*   - intros. exists ζ2. cbn - [Sub.comp]. now rewrite Sub.comp_id_left. *)
+    (*   - intros. constructor. *)
+    (*   - intros. constructor. *)
+    (*   - intros * IH1 IH2 *. cbn. *)
+    (*     (* apply (mg_bind (boxmgu s1 t1 ζ1) _ (cmgu s1 t1 (ζ1 ⊙ ζ2))); auto. *) *)
+    (* Admitted. *)
+
+    (* Lemma boxmgu_spec : BoxUnifierSpec boxmgu. *)
+    (* Proof. *)
+    (*   intros s t. pattern (boxmgu s t). *)
+    (*   apply boxmgu_elim; clear s t. *)
+    (*   - cbn. intros. apply boxflex_spec. *)
+    (*   - cbn. intros x xIn t w1 ζ1. *)
+    (*     generalize (boxflex_spec xIn t ζ1). cbn. *)
+    (*     apply option.spec_monotonic. *)
+    (*     + intros [w2 [ζ2 []]] H. *)
+    (*       now rewrite unifies_sym. *)
+    (*     + intros H. *)
+    (*       now rewrite unifies_sym. *)
+    (*   - constructor. apply trivialproblem. *)
+    (*   - constructor. discriminate. *)
+    (*   - constructor. discriminate. *)
+    (*   - cbn. intros. *)
+    (*     rewrite spec_μ. *)
+    (*     generalize (H w1 ζ1). clear H. *)
+    (*     apply option.spec_monotonic. *)
+    (*     intros [w2 [ζ2 _]] ?. *)
+    (*     rewrite spec_μ. *)
+    (*     generalize (H0 w2 (Tri.trans ζ1 ζ2)). clear H0. *)
+    (*     apply option.spec_monotonic. *)
+    (*     intros [w3 [ζ3 _]] ?. *)
+    (*     constructor. unfold four. *)
+    (*     + rewrite Tri.trans_refl, unifiesX_equiv; cbn. *)
+    (*       rewrite Sub.triangular_trans. *)
+    (*       rewrite Sub.triangular_trans in H0. *)
+    (*       now apply optimists_unifies. *)
+    (*     + admit. *)
+    (*     + admit. *)
+    (* Admitted. *)
+
+    Lemma boxmgu_sound (t1 t2 : Ty w) :
+      forall {w1} (ζ1 : w ⊒⁻ w1),
+        wlp
+          (boxmgu t1 t2 ζ1)
+          (fun w2 ζ2 _ => P.unifies t1[ζ1] t2[ζ1] ζ2).
+    Proof.
+      pattern (boxmgu t1 t2).
+      apply boxmgu_elim; clear t1 t2; cbn; intros; try (now constructor).
+      - destruct (boxflex_spec xIn t ζ1); constructor.
+        destruct a as [w2 [ζ2 []]]. apply H.
+      - destruct (boxflex_spec xIn t ζ1); constructor.
+        destruct a as [w2 [ζ2 []]]. apply unifies_sym. apply H.
+      - rewrite wlp_μ. generalize (H _ ζ1). clear H.
+        apply option.wlp_monotonic. intros [w2 [ζ2 _]] ?.
+        rewrite wlp_μ. generalize (H0 _ (ζ1 ⊙ ζ2)).
+        apply option.wlp_monotonic. intros [w3 [ζ3 _]] ?.
+        constructor. unfold four. cbn.
+        rewrite ?Sub.triangular_trans. cbn.
+        rewrite Sub.comp_id_right.
+        apply unifiesX_equiv. cbn.
+        split.
+        + revert H. apply dclosed_unifies. apply Sub.geq_extend.
+        + revert H1. unfold unifies.
+          now rewrite ?Sub.triangular_trans, ?Sub.subst_comp.
+    Qed.
+
+    Lemma boxmgu_complete (t1 t2 : Ty w) :
+      forall {w0} (ζ0 : w ⊒⁻ w0) [w1] (ζ1 : w0 ⊒ˢ w1),
+        P.unifies t1[ζ0] t2[ζ0] ζ1 ->
+        wp (boxmgu t1 t2 ζ0) (fun mgw mgζ _ => mgζ ≽ˢ ζ1).
+    Proof.
+      pattern (boxmgu t1 t2).
+      apply boxmgu_elim; clear t1 t2;
+        cbn - [Sub.subst]; intros; try (now constructor);
+        try discriminate.
+      - destruct (boxflex_spec xIn t ζ0).
+        + constructor. destruct a as [w2 [ζ2 []]]. now apply H0.
+        + now apply H0 in H.
+      - destruct (boxflex_spec xIn t ζ0).
+        + constructor. destruct a as [w2 [ζ2 []]]. now apply H0.
+        + now apply unifies_sym, H0 in H.
+      - constructor. apply Sub.geq_max.
+      - apply P.unifiesX_equiv in H1. destruct H1 as [HU1 HU2].
+        rewrite wp_μ. generalize (H _ ζ0 _ ζ1 HU1). clear H.
+        apply option.wp_monotonic. intros [mgw1 [mgζ1 _]] [ζ1' ->].
+        assert (P.unifies s2[ζ0 ⊙ mgζ1] t2[ζ0 ⊙ mgζ1] ζ1') as HU2'.
+        { revert HU2. unfold unifies.
+          now rewrite ?Sub.triangular_trans, ?Sub.subst_comp.
+        }
+        rewrite wp_μ. generalize (H0 _ (ζ0 ⊙ mgζ1) _ ζ1' HU2').
+        apply option.wp_monotonic. intros [mgw2 [mgζ2 _]] [ζ2' ->].
+        constructor. unfold four.
+        rewrite ?Sub.triangular_trans.
+        apply Sub.geq_precom.
+        apply Sub.geq_precom.
+        apply Sub.geq_max.
+    Qed.
+
+    Lemma boxmgu_spec' : BoxUnifierSpec boxmgu.
+    Proof.
+      unfold BoxUnifierSpec. intros *.
+      pose proof (boxmgu_complete t1 t2 ζ1) as Hcompl.
+      destruct (boxmgu_sound t1 t2 ζ1); constructor.
+      - destruct a as [w2 [ζ2 []]]. split; auto.
+        intros w3 ζ3 Hζ3. specialize (Hcompl w3 ζ3 Hζ3). revert Hcompl.
+        unfold wp. now rewrite option.wp_match.
+      - intros w3 ζ3 Hζ3. specialize (Hcompl w3 ζ3 Hζ3). revert Hcompl.
+        unfold wp. now rewrite option.wp_match.
+    Qed.
 
   End MguO.
 
-  Definition mgu : ⊢ Unifier :=
-    fun Σ s t => T (@Löb _ boxmgu Σ s t).
+  Definition bmgu : ⊢ BoxUnifier :=
+    fun w s t => Löb boxmgu _ s t.
 
-  Lemma mgu_complete {Σ} (s t : Ty Σ) {Σ2} (ζ2 : Σ ⊒ Σ2) (HU : ζ2 ⊨ s ~ t) :
-    wp (mgu s t) (fun Σ1 ζ1 _ => exists ζ12 : Σ1 ⊒ Σ2, ζ2 = Tri.trans ζ1 ζ12).
+  Definition mgu : ⊢ Unifier :=
+    fun w s t => T (@bmgu w s t).
+
+  Lemma bmgu_spec w : @BoxUnifierSpec w (@bmgu w).
   Proof.
-  Admitted.
+    pattern (@bmgu w). revert w. apply Löb_elim.
+    intros w IH. now apply boxmgu_spec'.
+  Qed.
+
+  Definition mgu_spec w : UnifierSpec (@mgu w).
+  Proof.
+    unfold UnifierSpec, mgu. intros t1 t2.
+    specialize (bmgu_spec t1 t2 Tri.refl).
+    apply option.spec_monotonic; cbn.
+    - intros [w1 [ζ1 []]]. now rewrite ?Sub.subst_id.
+    - now rewrite ?Sub.subst_id.
+  Qed.
+
+  Print Assumptions Löb_elim.
+  Print Assumptions bmgu_spec.
+
+  Definition boxsolve : ⊢ List (Prod Ty Ty) -> □◆Unit :=
+    fix solve {w} cs {struct cs} :=
+      match cs with
+      | List.nil => fun w1 ζ1 => η tt
+      | List.cons (t1,t2) cs =>
+          fun w1 ζ1 =>
+            ⟨ ζ2 ⟩ _ <- bmgu t1 t2 ζ1 ;;
+            solve cs _ (ζ1 ⊙ ζ2)
+         end.
+
+  Definition solve : ⊢ List (Prod Ty Ty) -> ◆Unit :=
+    fun w cs => boxsolve cs Tri.refl.
 
 End Variant1.
+Export Variant1.
 
 Module Variant2.
 
@@ -521,12 +1568,12 @@ Module Variant2.
     Ty -> Ty -> □◆Ty.
 
   Definition flex : ⊢ Ty -> ∀ x, In x -> ◆Ty :=
-    fun Σ t x xIn =>
+    fun w t x xIn =>
       match t with
-      | t_evar yIn =>
+      | Ty_hole yIn =>
           match occurs_check_view xIn yIn with
-          | Same _      => η (t_evar xIn)
-          | Diff _ yIn' => Some (sooner2diamond (x; (xIn; (t_evar yIn', t_evar yIn'))))
+          | Same _      => η (Ty_hole xIn)
+          | Diff _ yIn' => Some (sooner2diamond (x; (xIn; (Ty_hole yIn', Ty_hole yIn'))))
           end
       | _ => option_map
                (fun t' => sooner2diamond (x; (xIn; (t', t'))))
@@ -535,24 +1582,57 @@ Module Variant2.
 
   Section MguO.
 
-    Context [Σ] (lmgu : ▻BoxUnifier Σ).
+    Context [w] (lmgu : ▻BoxUnifier w).
 
-    Definition boxflex {x} (xIn : x ∈ Σ) (t : Ty Σ) : □◆Ty Σ :=
-      box_intro_split (flex t xIn) (fun z zIn u => lmgu _ (t_evar xIn)[z↦u] t[z↦u]).
+    Definition boxflex {x} (xIn : x ∈ w) (t : Ty w) : □◆Ty w :=
+      box_intro_split
+        (flex t xIn)
+        (fun z zIn u =>
+           let ζ := Sub.thick zIn u in
+           lmgu _ (Ty_hole xIn)[ζ] t[ζ]).
 
-    Equations boxmgu : BoxUnifier Σ :=
-    | t_evar xIn   | t            := boxflex xIn t;
-    | s            | t_evar yIn   := boxflex yIn s;
-    | t_bool       | t_bool       := fun _ _ => η t_bool;
-    | t_func s1 s2 | t_func t1 t2 := fun _ ζ1 =>
+    Equations boxmgu : BoxUnifier w :=
+    | Ty_hole xIn   | t            := boxflex xIn t;
+    | s            | Ty_hole yIn   := boxflex yIn s;
+    | Ty_bool       | Ty_bool       := fun _ _ => η Ty_bool;
+    | Ty_func s1 s2 | Ty_func t1 t2 := fun _ ζ1 =>
                                        ⟨ ζ2 ⟩ r1 <- boxmgu s1 t1 ζ1 ;;
                                        ⟨ ζ3 ⟩ r2 <- boxmgu s2 t2 (Tri.trans ζ1 ζ2) ;;
-                                       η (t_func (realsubst_slow r1 ζ3) r2);
+                                       η (Ty_func (realsubst_slow r1 ζ3) r2);
     | _            | _            := fun _ _ => None.
 
   End MguO.
 
   Definition mgu : ⊢ Unifier :=
-    fun Σ s t => T (@Löb _ boxmgu Σ s t).
+    fun w s t => T (@Löb _ boxmgu w s t).
+
 
 End Variant2.
+
+Fixpoint applyassign {w} (t : Ty w) (ass : Assignment w) : ty.
+Admitted.
+
+Fixpoint compose {w0 w1} (ζ : w0 ⊒⁻ w1) : Assignment w1 -> Assignment w0 :=
+  match ζ in (_ ⊒⁻ c) return (Assignment c -> Assignment w0) with
+  | Tri.refl => fun ass : Assignment w0 => ass
+  | @Tri.cons _ w' x xIn t ζ =>
+      fun ass  =>
+        let ass' := compose ζ ass in
+        env.insert xIn ass' (applyassign t ass')
+  end.
+
+Definition compose' {w0 w1} (ζ : w0 ⊒⁻ w1) : Assignment w1 -> Assignment w0.
+Proof.
+  intros ass.
+  apply env.tabulate.
+  intros x xIn.
+  apply (applyassign (env.lookup (Sub.triangular ζ) xIn) ass).
+Defined.
+
+Definition SubstLifted (A : Type) :
+  ⊢ Lifted A -> □(Lifted A).
+Proof.
+  unfold Valid, Box, Impl, Lifted.
+  intros w fa w1 ζ1 ass. apply fa.
+  apply (compose ζ1 ass).
+Defined.
